src/Disk.v
@@ -1,4 +1,4 @@
-Require Import List SepLogic BaseTypes.
+Require Import List Memx BaseTypes.
 Import ListNotations.
 
 Set Implicit Arguments.
@@ -6,25 +6,25 @@ Set Implicit Arguments.
 Section Disk.
   (* maybe rename better *)
   Definition valueset := (sealed_value * list sealed_value)%type.
-  Definition disk := @mem addr valueset.
+  Definition disk := @mem addr addr_dec valueset.
 
   Definition upd_disk := @upd addr valueset addr_dec.
 
   Definition read (d: disk) (a: addr) :=
-    match mem_read d a with
+    match d a with
     | None => None
     | Some vs => Some (fst vs)
     end.
   
   Definition write (d: disk) (a: addr) (v: sealed_value) : disk :=
-    match mem_read d a with
+    match d a with
     | None => d
     | Some vs => upd_disk d a (v, fst vs::snd vs)
     end.
 
 
   Definition sync (d: disk) (a: addr) : disk :=
-    match mem_read d a with
+    match d a with
     | None => d
     | Some vs => upd_disk d a (fst vs, [])
     end.
@@ -36,7 +36,7 @@ End Disk.
 
 Section Store.
   
-  Definition store := @mem handle sealed_value.
+  Definition store := @mem handle handle_dec sealed_value.
   Definition upd_store := @upd handle sealed_value handle_dec.
   
 End Store.
