src/Hoare.v
@@ -1,17 +1,15 @@
 Require Import BaseTypes Prog ProgAuto.
-Require Import Disk SepLogic.
-Import PredNotations.
-Open Scope pred_scope.
+Require Import Disk Memx Predx SepAuto.
 
 Set Implicit Arguments.
 
 
 (** ** Hoare logic *)
-Definition precond := user -> oracle ->  store -> @pred addr valueset.
+Definition precond := user -> oracle ->  store -> @pred addr addr_dec valueset.
 Definition postcond {T: Type} := user -> oracle ->  store ->
-                                 oracle -> store -> T -> @pred addr valueset.
+                                 oracle -> store -> T -> @pred addr addr_dec valueset.
 Definition crashcond := user -> oracle ->  store ->
-                        oracle -> store -> @pred addr valueset.
+                        oracle -> store -> @pred addr addr_dec valueset.
 
 Definition can_exec {T: Type} (pre: precond) (p: prog T):=
   forall u o d s,
@@ -26,39 +24,58 @@ Definition hoare_triple {T: Type} (pre: precond) (p: prog T) (post: @postcond T)
          ret = Finished o' d' s' r
          /\ post u o s o' s' r d') \/
      (exists o' d' s',
-        ret = Crashed _ o' d' s' /\ crash u o s o' s' d')) /\
+        ret = Crashed _ o' d' s' /\ crash u o s o' s' d'))%type /\
     trace_ok tr.
+
 
 Notation
   "<< u , o , s >> pre p" :=
-  (forall F, can_exec (fun (u:user) (o:oracle) (s: store) => F * pre) p)
+  (forall F, can_exec (fun (u:user) (o:oracle) (s: store) => F * pre)%pred p)
     (at level 10, u at next level, o at next level, s at next level, pre at next level, p at next level,
-     format "'[v  ' '<<' u ','  o ','  s '>>' '//' '[' pre ']' '//' '[' p ']' ']'").
+     format "'[v' '[  ' '<<' u ','  o ','  s '>>' '//' pre '//' p ']' ']'").
 
 
   
 Notation
   "<< u , o , s >> pre p << o' , s' , r >> post crash" :=
-  (forall F, hoare_triple (fun (u:user) (o:oracle) (s: store) => F * pre) p (fun (u:user) (o:oracle) (s: store) (o':oracle) (s': store) r => F * post ) (fun u (o:oracle) (s: store) o' s' => F * crash))
+  (forall F, hoare_triple
+          (fun (u:user) (o:oracle) (s: store) => F * pre)%pred
+          p
+          (fun (u:user) (o:oracle) (s: store) (o':oracle) (s': store) r => F * post)%pred
+          (fun u (o:oracle) (s: store) o' s' => F * crash)%pred)
     (at level 10, u at next level, o at next level, s at next level, pre at next level, p at next level, o' at next level, s' at next level, r at next level, post at next level, crash at next level,
      format "'[v' '[  ' '<<' u ','  o ','  s '>>' '//' '[' pre ']' '//' '[' p ']' ']' '//' '[  ' '<<' o' ','  s' ','  r '>>' '//' '[' post ']' '//' '[' crash ']' ']' ']'").
 
-Example read_can_exec:
-  forall a v,
-    << u, o, s >>
-      (a |-> v)
-      (Read a).
-Proof. intros. Abort.
+Notation
+  "{{ e1 }} << u , o , s >> pre p << o' , s' , r >> post crash" :=
+   (exists e1, (forall F, hoare_triple
+          (fun (u:user) (o:oracle) (s: store) => F * pre)%pred
+          p
+          (fun (u:user) (o:oracle) (s: store) (o':oracle) (s': store) r => F * post)%pred
+          (fun u (o:oracle) (s: store) o' s' => F * crash)%pred))
+    (at level 10, u at next level, o at next level, s at next level, pre at next level, p at next level, o' at next level, s' at next level, r at next level, post at next level, crash at next level,
+     format "'[v' '{{' e1 '}}' '//' '[  ' '<<' u ','  o ','  s '>>' '//' pre '//' p ']' '//' '[  ' '<<' o' ','  s' ','  r '>>' '//' post '//' crash ']' ']'").
 
-Example read_spec:
-  forall a v,
-    <<u, o, s>>
-      (a |-> v)
-      (Read a)
-    << o', s', r >>
-      ([s' r = Some (fst v)] * a |-> v)
-      (a |-> v).
-Proof. intros. Abort.
+Notation
+  "{{ e1 e2 }} << u , o , s >> pre p << o' , s' , r >> post crash" :=
+   (exists e1 e2, (forall F, hoare_triple
+          (fun (u:user) (o:oracle) (s: store) => F * pre)%pred
+          p
+          (fun (u:user) (o:oracle) (s: store) (o':oracle) (s': store) r => F * post)%pred
+          (fun u (o:oracle) (s: store) o' s' => F * crash)%pred))
+    (at level 10, u at next level, o at next level, s at next level, pre at next level, p at next level, o' at next level, s' at next level, r at next level, post at next level, crash at next level,
+     format  "'[v' '{{' e1 e2 '}}' '//' '[  ' '<<' u ','  o ','  s '>>' '//' pre '//' p ']' '//' '[  ' '<<' o' ','  s' ','  r '>>' '//' post '//' crash ']' ']'").
+
+
+Notation
+  "{{ e1 e2 e3 }} << u , o , s >> pre p << o' , s' , r >> post crash" :=
+   (exists e1 e2 e3, (forall F, hoare_triple
+          (fun (u:user) (o:oracle) (s: store) => F * pre)%pred
+          p
+          (fun (u:user) (o:oracle) (s: store) (o':oracle) (s': store) r => F * post)%pred
+          (fun u (o:oracle) (s: store) o' s' => F * crash)%pred))
+    (at level 10, u at next level, o at next level, s at next level, pre at next level, p at next level, o' at next level, s' at next level, r at next level, post at next level, crash at next level,
+     format  "'[v' '{{' e1 e2 e3 '}}' '//' '[  ' '<<' u ','  o ','  s '>>' '//' pre '//' p ']' '//' '[  ' '<<' o' ','  s' ','  r '>>' '//' post '//' crash ']' ']'").
 
 
 Definition complete {T: Type} (pre: precond) (p: prog T) (post: postcond) (crash: crashcond):=
@@ -67,7 +84,7 @@ Definition complete {T: Type} (pre: precond) (p: prog T) (post: postcond) (crash
 Theorem can_exec_strengthen_pre:
   forall T (p: prog T) (pre pre': precond),
   can_exec pre p ->
-  (forall  u o s, pre' u o s ===>  pre u o s) ->
+  (forall  u o s, pre' u o s =p=>  pre u o s) ->
   can_exec pre' p.
 Proof.
   unfold complete, can_exec; intros;
@@ -78,7 +95,7 @@ Qed.
 Theorem hoare_triple_strengthen_pre:
   forall T (p: prog T) (pre pre': precond) post crash,
   hoare_triple pre p post crash ->
-  (forall  u o s, pre' u o s ===>  pre u o s) ->
+  (forall  u o s, pre' u o s =p=>  pre u o s) ->
   hoare_triple pre' p post crash.
 Proof.
   unfold complete, hoare_triple; intros;
@@ -89,7 +106,7 @@ Qed.
 Theorem complete_strengthen_pre:
   forall T (p: prog T) (pre pre': precond) post crash,
   complete pre p post crash ->
-  (forall  u o s, pre' u o s ===>  pre u o s) ->
+  (forall  u o s, pre' u o s =p=>  pre u o s) ->
   complete pre' p post crash.
 Proof.
   unfold complete, can_exec, hoare_triple; intros;
@@ -139,7 +156,7 @@ Theorem hoare_triple_weaken_post_strong:
   forall T (p: prog T) pre (post post': postcond) crash,
   hoare_triple pre p post crash ->
   (forall  u o s o' s' (r: T),
-      post u o s o' s' r ===>
+      post u o s o' s' r =p=>
       post' u o s o' s' r) ->
   hoare_triple pre p post' crash.
 Proof.
@@ -152,7 +169,7 @@ Theorem complete_weaken_post_strong:
   forall T (p: prog T) pre (post post': postcond) crash,
   complete pre p post crash ->
   (forall  u o s o' s' (r: T),
-      post u o s o' s' r ===>
+      post u o s o' s' r =p=>
       post' u o s o' s' r) ->
   complete pre p post' crash.
 Proof.
@@ -198,7 +215,7 @@ Qed.
 Theorem hoare_triple_weaken_crash_strong:
   forall T (p: prog T) pre post (crash crash': crashcond),
   hoare_triple pre p post crash ->
-  (forall  u o s o' s', crash u o s o' s' ===> crash' u o s o' s') ->
+  (forall  u o s o' s', crash u o s o' s' =p=> crash' u o s o' s') ->
   hoare_triple pre p post crash'.
 Proof.
   intros; eapply hoare_triple_weaken_crash_weak; eauto.
@@ -208,12 +225,206 @@ Qed.
 Theorem complete_weaken_crash_strong:
   forall T (p: prog T) pre post (crash crash': crashcond),
   complete pre p post crash ->
-  (forall  u o s o' s', crash u o s o' s' ===> crash' u o s o' s') ->
+  (forall  u o s o' s', crash u o s o' s' =p=> crash' u o s o' s') ->
   complete pre p post crash'.
 Proof.
   intros; eapply complete_weaken_crash_weak; eauto.
   intros; eapply H0; eauto.
 Qed.
+
+Theorem hoare_triple_pimpl_strong :
+    forall T1 T2 (p1: prog T1) (p2: T1 -> prog T2) pre1 pre2 post1 post2 crash1 crash2,
+      hoare_triple pre1 p1 post1 crash1 ->
+      (forall r, hoare_triple pre2 (p2 r) post2 crash2) ->
+    (forall  u o d s o' d' s' r tr,
+      pre1 u o s d ->
+      exec u o d s p1 (Finished o' d' s' r) tr ->
+      post1 u o s o' s' r d' ->
+      pre2 u o' s' d') ->
+    (forall u o d s o' d' s' tr,
+      pre1 u o s d ->
+      exec u o d s p1 (Crashed _ o' d' s') tr ->
+      crash1 u o s o' s' d' ->
+      crash2 u o s o' s' d') ->
+    (forall  u o s o' d' s' o'' s'' d'' r r2 tr,
+      post1 u o s o' s' r d' ->
+      pre2 u o' s' d' ->
+      exec u o' d' s' (p2 r) (Finished o'' d'' s'' r2) tr ->
+      post2 u o s o'' s'' r2 d'') ->
+    (forall  u o s o' d' s' o'' s'' d'' r tr,
+      post1 u o s o' s' r d' ->
+      pre2 u o' s' d' ->
+      exec u o' d' s' (p2 r) (Crashed _ o'' d'' s'') tr ->
+      crash2 u o s o'' s'' d'') ->
+    hoare_triple pre1 (Bind p1 p2) post2 crash2.
+Proof.
+  unfold complete, can_exec, hoare_triple; intros.
+  inv_exec_perm.
+  {
+      edestruct H; eauto.
+      destruct H8; cleanup.
+      edestruct H0; eauto.
+      destruct H8; eauto; cleanup; eauto.
+      split. left.
+      repeat eexists; eauto.
+      apply trace_ok_app; eauto.
+    }
+    {
+      destruct H6.
+      - edestruct H; eauto; destruct H7; cleanup.
+        split; eauto; right; repeat eexists; eauto.
+      - cleanup.
+        edestruct H; eauto; destruct H8; cleanup.
+        edestruct H0; eauto.
+        destruct H8; eauto; cleanup; eauto.
+        split. right.
+        repeat eexists; eauto.
+        apply trace_ok_app; eauto.
+    }
+Qed.
+
+Theorem hoare_triple_pimpl' :
+    forall T1 T2 (p1: prog T1) (p2: T1 -> prog T2) pre1 post1 post2 crash1 crash2,
+      hoare_triple pre1 p1 post1 crash1 ->
+      (forall r, hoare_triple (fun u o' s' => exists o s d, [[pre1 u o s d]] * post1 u o s o' s' r)%pred (p2 r) post2 crash2) ->
+    (forall u o d s o' d' s' tr,
+      pre1 u o s d ->
+      exec u o d s p1 (Crashed _ o' d' s') tr ->
+      crash1 u o s o' s' d' ->
+      crash2 u o s o' s' d') ->
+    (forall  u o s o' d' s' o'' s'' d'' r r2 tr,
+      post1 u o s o' s' r d' ->
+      exec u o' d' s' (p2 r) (Finished o'' d'' s'' r2) tr ->
+      post2 u o s o'' s'' r2 d'') ->
+    (forall  u o s o' d' s' o'' s'' d'' r tr,
+      post1 u o s o' s' r d' ->
+      exec u o' d' s' (p2 r) (Crashed _ o'' d'' s'') tr ->
+      crash2 u o s o'' s'' d'') ->
+    hoare_triple pre1 (Bind p1 p2) post2 crash2.
+Proof.
+  unfold hoare_triple; intros.
+  inv_exec_perm.
+  {
+      edestruct H; eauto.
+      destruct H7; cleanup.
+      edestruct H0; eauto.
+      pred_apply; cancel; eauto.
+      destruct H7; eauto; cleanup; eauto.
+      split. left.
+      repeat eexists; eauto.
+      apply trace_ok_app; eauto.
+    }
+    {
+      destruct H5.
+      - edestruct H; eauto; destruct H6; cleanup.
+        split; eauto; right; repeat eexists; eauto.
+      - cleanup.
+        edestruct H; eauto; destruct H7; cleanup.
+        edestruct H0; eauto.
+        pred_apply; cancel; eauto.
+        destruct H7; eauto; cleanup; eauto.
+        split. right.
+        repeat eexists; eauto.
+        apply trace_ok_app; eauto.
+    }
+Qed.
+
+Theorem hoare_triple_pimpl'' :
+    forall T1 T2 (p1: prog T1) (p2: T1 -> prog T2) pre1 post1 post2 crash1 crash2,
+      hoare_triple pre1 p1 post1 crash1 ->
+      (forall u o s d r,
+          pre1 u o s d ->
+          hoare_triple (fun u' o' s' => [[u = u']] * post1 u' o s o' s' r)%pred (p2 r) post2 crash2) ->
+    (forall u o d s o' d' s' tr,
+      pre1 u o s d ->
+      exec u o d s p1 (Crashed _ o' d' s') tr ->
+      crash1 u o s o' s' d' ->
+      crash2 u o s o' s' d') ->
+    (forall  u o s o' d' s' o'' s'' d'' r r2 tr,
+      post1 u o s o' s' r d' ->
+      exec u o' d' s' (p2 r) (Finished o'' d'' s'' r2) tr ->
+      post2 u o s o'' s'' r2 d'') ->
+    (forall  u o s o' d' s' o'' s'' d'' r tr,
+      post1 u o s o' s' r d' ->
+      exec u o' d' s' (p2 r) (Crashed _ o'' d'' s'') tr ->
+      crash2 u o s o'' s'' d'') ->
+    hoare_triple pre1 (Bind p1 p2) post2 crash2.
+Proof.
+  unfold hoare_triple; intros.
+  inv_exec_perm.
+  {
+      edestruct H; eauto.
+      destruct H7; cleanup.
+      edestruct H0; eauto.
+      pred_apply; cancel; eauto.
+      destruct H7; eauto; cleanup; eauto.
+      split. left.
+      repeat eexists; eauto.
+      apply trace_ok_app; eauto.
+    }
+    {
+      destruct H5.
+      - edestruct H; eauto; destruct H6; cleanup.
+        split; eauto; right; repeat eexists; eauto.
+      - cleanup.
+        edestruct H; eauto; destruct H7; cleanup.
+        edestruct H0; eauto.
+        pred_apply; cancel; eauto.
+        destruct H7; eauto; cleanup; eauto.
+        split. right.
+        repeat eexists; eauto.
+        apply trace_ok_app; eauto.
+    }
+Qed.
+
+
+Theorem hoare_triple_pimpl :
+    forall T1 T2 (p1: prog T1) (p2: T1 -> prog T2) pre1 post1 post2 crash1 crash2,
+      hoare_triple pre1 p1 post1 crash1 ->
+      (forall u o s d r,
+          pre1 u o s d ->
+          hoare_triple (fun u' o' s' => [[u = u']] * post1 u' o s o' s' r)%pred (p2 r) post2 crash2) ->
+    (forall u o d s o' s',
+      pre1 u o s d ->
+      crash1 u o s o' s' =p=> crash2 u o s o' s') ->
+    (forall  u o s o' d' s' o'' s'' r r2,
+      post1 u o s o' s' r d' ->
+      post2 u o' s' o'' s'' r2 =p=> post2 u o s o'' s'' r2) ->
+    (forall  u o s o' d' s' o'' s'' r,
+      post1 u o s o' s' r d' ->
+      crash2 u o' s' o'' s'' =p=> crash2 u o s o'' s'') ->
+    hoare_triple pre1 (Bind p1 p2) post2 crash2.
+Proof.
+  unfold hoare_triple; intros.
+  inv_exec_perm.
+  {
+      edestruct H; eauto.
+      destruct H7; cleanup.
+      edestruct H0; eauto.
+      pred_apply; cancel; eauto.
+      destruct H7; eauto; cleanup; eauto.
+      split. left.
+      repeat eexists; eauto.
+      eapply H2; eauto.
+      apply trace_ok_app; eauto.
+    }
+    {
+      destruct H5.
+      - edestruct H; eauto; destruct H6; cleanup.
+        split; eauto; right; repeat eexists; eauto.
+        eapply H1; eauto.
+      - cleanup.
+        edestruct H; eauto; destruct H7; cleanup.
+        edestruct H0; eauto.
+        pred_apply; cancel; eauto.
+        destruct H7; eauto; cleanup; eauto.
+        split. right.
+        repeat eexists; eauto.
+        eapply H3; eauto.
+        apply trace_ok_app; eauto.
+    }
+Qed.
+
 
 Theorem complete_pimpl_strong :
     forall T1 T2 (p1: prog T1) (p2: T1 -> prog T2) pre1 pre2 post1 post2 crash1 crash2,
