src/Errno.v
@@ -1,0 +1,26 @@
+Set Implicit Arguments.
+
+Inductive Errno :=
+| ELOGOVERFLOW
+| ENOTDIR
+| EISDIR
+| ENOENT
+| EFBIG
+| ENAMETOOLONG
+| EEXIST
+| ENOSPCBLOCK
+| ENOSPCINODE
+| ENOTEMPTY
+| EINVAL
+| ENOPERMIT.
+
+Inductive res (T : Type) :=
+| OK : T -> res T
+| Err : Errno -> res T.
+
+Arguments Err {T} _.
+
+Inductive isError : forall {T : Type}, res T -> Prop :=
+| isErrorErr : forall T errno, @isError T (Err errno).
+
+Hint Constructors isError.
