src/SimpleDisk.v
@@ -1,0 +1,417 @@
+Require Import Primitives Omega.
+Open Scope pred_scope.
+
+Axiom nat_to_value : nat -> value.
+Axiom value_to_nat : value -> nat.
+Axiom nat_to_value_to_nat:
+  forall n, value_to_nat (nat_to_value n) = n.
+Axiom value_to_nat_to_value:
+  forall v, nat_to_value (value_to_nat v) = v.
+
+Definition rep (dh: @mem addr addr_dec sealed_value) : @pred addr addr_dec Disk.valueset :=
+  exists bitmap bl val1 val2,
+    (0 |-> ((Public, bitmap), bl) *
+     1 |-> val1 * 2 |-> val2 *
+     [[value_to_nat bitmap < 4]] *
+     [[dh 0 = None]] *
+     [[value_to_nat bitmap = 0 ->
+      dh 1 = None /\ dh 2 = None]] *
+     [[value_to_nat bitmap = 1 ->
+      dh 1 = Some (fst val1) /\ dh 2 = None]] *
+     [[value_to_nat bitmap = 2 ->
+      dh 1 = None /\ dh 2 = Some (fst val2)]] *
+     [[value_to_nat bitmap = 3 ->
+      dh 1 = Some (fst val1) /\ dh 2 = Some (fst val2)]] *
+     [[forall n, n > 2 -> dh n = None]]).
+
+Definition alloc : prog (option addr) :=
+  sv <- Read 0;
+  v <- Unseal sv;
+  if addr_dec (value_to_nat v) 0 then
+    zv <- Seal Public (nat_to_value 0);
+    _ <- Write 1 zv;
+    sh <- Seal Public (nat_to_value 1);
+    _ <- Write 0 sh;
+    Ret (Some 1)
+  else if addr_dec (value_to_nat v) 1 then
+    zv <- Seal Public (nat_to_value 0);
+    _ <- Write 2 zv;
+    sh <- Seal Public (nat_to_value 3);
+    _ <- Write 0 sh;
+    Ret (Some 2)
+  else if addr_dec (value_to_nat v) 2 then
+    zv <- Seal Public (nat_to_value 0);
+    _ <- Write 1 zv;
+    sh <- Seal Public (nat_to_value 3);
+    _ <- Write 0 sh;
+    Ret (Some 1)
+  else
+    Ret None.
+
+Definition read a : prog (option handle) :=
+  if addr_dec a 1 then
+    sv <- Read 0;
+    v <- Unseal sv;
+    if addr_dec (value_to_nat v) 1 then
+      h <- Read a;
+      Ret (Some h)
+    else if addr_dec (value_to_nat v) 3 then
+      h <- Read a;
+      Ret (Some h)
+    else
+      Ret None
+  else if addr_dec a 2 then
+    sv <- Read 0;
+    v <- Unseal sv;
+    if addr_dec (value_to_nat v) 2 then
+      h <- Read a;
+      Ret (Some h)
+    else if addr_dec (value_to_nat v) 3 then
+      h <- Read a;
+      Ret (Some h)
+    else
+      Ret None
+  else
+    Ret None.
+
+Definition write a h : prog (option unit) :=
+  if addr_dec a 1 then
+    sv <- Read 0;
+    v <- Unseal sv;
+    if addr_dec (value_to_nat v) 1 then
+      _ <- Write a h;
+      Ret (Some tt)
+    else if addr_dec (value_to_nat v) 3 then
+      h <- Write a h;
+      Ret (Some tt)
+    else
+      Ret None
+  else if addr_dec a 2 then
+    sv <- Read 0;
+    v <- Unseal sv;
+    if addr_dec (value_to_nat v) 2 then
+      h <- Write a h;
+      Ret (Some tt)
+    else if addr_dec (value_to_nat v) 3 then
+      h <- Write a h;
+      Ret (Some tt)
+    else
+      Ret None
+  else
+    Ret None.
+
+Definition free a : prog unit :=
+  if addr_dec a 1 then
+    sv <- Read 0;
+    v <- Unseal sv;
+    if addr_dec (value_to_nat v) 1 then
+      sh <- Seal Public (nat_to_value 0);
+      Write 0 sh
+    else if addr_dec (value_to_nat v) 3 then
+      sh <- Seal Public (nat_to_value 2);
+      Write 0 sh
+    else
+      Ret tt
+  else if addr_dec a 2 then
+    sv <- Read 0;
+    v <- Unseal sv;
+    if addr_dec (value_to_nat v) 2 then
+      sh <- Seal Public (nat_to_value 0);
+      Write 0 sh
+    else if addr_dec (value_to_nat v) 3 then
+      sh <- Seal Public (nat_to_value 1);
+      Write 0 sh
+    else
+      Ret tt
+  else
+    Ret tt.
+
+
+Theorem hoare_triple_pre_ex':
+  forall T V (p: prog T) pre post crash,
+  (forall (v: V), hoare_triple (fun a b c => pre v a b c) p post crash) ->
+  hoare_triple (fun a b c => exists (v: V), pre v a b c) p post crash.
+Proof.
+  unfold hoare_triple; intros.
+  destruct_lift H0; cleanup.
+  eapply H; eauto.
+Qed.
+
+Theorem hoare_triple_pre_ex:
+  forall T V (p: prog T) pre post crash F,
+  (forall (v: V), hoare_triple (fun a b c => F * pre v a b c) p post crash) ->
+  hoare_triple (fun a b c => F * exists (v: V), pre v a b c) p post crash.
+Proof.
+  intros.
+  eapply hoare_triple_strengthen_pre.
+  apply hoare_triple_pre_ex'.
+  instantiate (1:= fun v a b c => F * pre v a b c).
+  simpl; eauto.
+  intros; cancel.
+Qed.
+
+
+Lemma upd_eq':
+  forall (A V : Type) (AEQ : EqDec A) (m : mem) (a : A) (v : V),
+    @upd _ _ AEQ m a v a = Some v.
+Proof.
+  intros; apply upd_eq; eauto.
+Qed.
+
+
+Theorem alloc_ok:
+  forall dh,
+  << u, o, s >>
+   (rep dh)
+   (alloc)
+  << o', s', r >>
+   (exists dh',
+    rep dh' *
+     [[(r = None /\ dh' = dh) \/
+       (exists h, r = Some h /\ dh' = upd dh h (Public, nat_to_value 0) /\ dh h = None)%type]])
+   (exists dh',
+    rep dh' *
+     [[(dh' = dh) \/
+       (exists h, dh' = upd dh h (Public, nat_to_value 0) /\ dh h = None)%type]]).
+Proof.
+  intros.
+  unfold alloc; simpl.
+  unfold rep.
+  repeat (apply hoare_triple_pre_ex; intros).
+
+  eapply hoare_triple_pimpl;
+  try solve [intros; simpl in *; eauto].
+  eapply hoare_triple_strengthen_pre;
+  [apply read_okay | intros; simpl; cancel].
+
+  intros; simpl.
+  eapply hoare_triple_pimpl;
+  try solve [intros; simpl in *; eauto].
+  eapply hoare_triple_strengthen_pre;
+  [apply unseal_okay | intros; simpl; cancel].
+  apply upd_eq; eauto.
+  simpl; apply can_access_public.
+  
+  intros; simpl.
+  destruct (addr_dec (value_to_nat r0) 0); simpl.
+  {
+    eapply hoare_triple_pimpl;
+    try solve [intros; simpl in *; eauto].
+    eapply hoare_triple_strengthen_pre;
+    [apply seal_okay | intros; simpl; cancel].
+
+    intros; simpl. 
+    eapply hoare_triple_pimpl;
+    try solve [intros; simpl in *; eauto].
+    eapply hoare_triple_strengthen_pre;
+    [apply write_okay | intros; simpl; cancel].
+    apply upd_eq; eauto.
+
+    intros; simpl.
+    destruct_pairs.
+    eapply hoare_triple_pimpl;
+    try solve [intros; simpl in *; eauto].
+    eapply hoare_triple_strengthen_pre;
+    [apply seal_okay | intros; simpl; cancel].
+
+    intros; simpl. 
+    eapply hoare_triple_pimpl;
+    try solve [intros; simpl in *; eauto].
+    eapply hoare_triple_strengthen_pre;
+    [apply write_okay | intros; simpl; cancel].
+    apply upd_eq; eauto.
+
+    {
+      intros; simpl.
+      eapply hoare_triple_strengthen_pre.
+      eapply hoare_triple_weaken_post_strong.
+      eapply hoare_triple_weaken_crash_strong.
+      apply ret_okay.  
+      3: intros; simpl; cancel.
+      
+      intros; simpl;
+        norm; [cancel|].
+      eassign (upd dh 1 (Public, nat_to_value 0)).
+      rewrite nat_to_value_to_nat; eauto.
+      rewrite upd_eq'.
+      repeat rewrite upd_ne; eauto.
+      destruct_lift H;
+        destruct_lift H1; cleanup.
+      intuition (eauto; try omega).
+      rewrite upd_ne; eauto.
+      omega.
+
+      intros; simpl.
+      norm; [cancel|].
+      eassign (upd dh 1 (Public, nat_to_value 0)).
+      rewrite nat_to_value_to_nat; eauto.
+      rewrite upd_eq'.
+      repeat rewrite upd_ne; eauto.
+      destruct_lift H;
+        destruct_lift H1; cleanup.
+      intuition (eauto; try omega).
+      rewrite upd_ne; eauto.
+      omega.
+    }
+    all: try solve [
+      intros; simpl in *;
+      destruct_lift H;
+        destruct_lift H1; cleanup;
+      cancel; eauto].      
+  }
+  destruct (addr_dec (value_to_nat r0) 1); simpl.
+  {
+    eapply hoare_triple_pimpl;
+    try solve [intros; simpl in *; eauto].
+    eapply hoare_triple_strengthen_pre;
+    [apply seal_okay | intros; simpl; cancel].
+
+    intros; simpl. 
+    eapply hoare_triple_pimpl;
+    try solve [intros; simpl in *; eauto].
+    eapply hoare_triple_strengthen_pre;
+    [apply write_okay | intros; simpl; cancel].
+    apply upd_eq; eauto.
+
+    intros; simpl.
+    destruct_pairs.
+    eapply hoare_triple_pimpl;
+    try solve [intros; simpl in *; eauto].
+    eapply hoare_triple_strengthen_pre;
+    [apply seal_okay | intros; simpl; cancel].
+
+    intros; simpl. 
+    eapply hoare_triple_pimpl;
+    try solve [intros; simpl in *; eauto].
+    eapply hoare_triple_strengthen_pre;
+    [apply write_okay | intros; simpl; cancel].
+    apply upd_eq; eauto.
+
+    {
+      intros; simpl.
+      eapply hoare_triple_strengthen_pre.
+      eapply hoare_triple_weaken_post_strong.
+      eapply hoare_triple_weaken_crash_strong.
+      apply ret_okay.  
+      3: intros; simpl; cancel.
+      
+      intros; simpl;
+        norm; [cancel|].
+      eassign (upd dh 2 (Public, nat_to_value 0)).
+      rewrite nat_to_value_to_nat; eauto.
+      rewrite upd_eq'.
+      repeat rewrite upd_ne; eauto.
+      destruct_lift H;
+        destruct_lift H1; cleanup.
+      intuition (eauto; try omega).
+      rewrite upd_ne; eauto.
+      omega.
+
+      intros; simpl.
+      norm; [cancel|].
+      eassign (upd dh 2 (Public, nat_to_value 0)).
+      rewrite nat_to_value_to_nat; eauto.
+      rewrite upd_eq'.
+      repeat rewrite upd_ne; eauto.
+      destruct_lift H;
+        destruct_lift H1; cleanup.
+      intuition (eauto; try omega).
+      rewrite upd_ne; eauto.
+      omega.
+    }
+    all: try solve [
+      intros; simpl in *;
+      destruct_lift H;
+        destruct_lift H1; cleanup;
+      cancel; eauto].      
+  }
+  destruct (addr_dec (value_to_nat r0) 2); simpl.
+  {
+    eapply hoare_triple_pimpl;
+    try solve [intros; simpl in *; eauto].
+    eapply hoare_triple_strengthen_pre;
+    [apply seal_okay | intros; simpl; cancel].
+
+    intros; simpl. 
+    eapply hoare_triple_pimpl;
+    try solve [intros; simpl in *; eauto].
+    eapply hoare_triple_strengthen_pre;
+    [apply write_okay | intros; simpl; cancel].
+    apply upd_eq; eauto.
+
+    intros; simpl.
+    destruct_pairs.
+    eapply hoare_triple_pimpl;
+    try solve [intros; simpl in *; eauto].
+    eapply hoare_triple_strengthen_pre;
+    [apply seal_okay | intros; simpl; cancel].
+
+    intros; simpl. 
+    eapply hoare_triple_pimpl;
+    try solve [intros; simpl in *; eauto].
+    eapply hoare_triple_strengthen_pre;
+    [apply write_okay | intros; simpl; cancel].
+    apply upd_eq; eauto.
+
+    {
+      intros; simpl.
+      eapply hoare_triple_strengthen_pre.
+      eapply hoare_triple_weaken_post_strong.
+      eapply hoare_triple_weaken_crash_strong.
+      apply ret_okay.  
+      3: intros; simpl; cancel.
+      
+      intros; simpl;
+        norm; [cancel|].
+      eassign (upd dh 1 (Public, nat_to_value 0)).
+      rewrite nat_to_value_to_nat; eauto.
+      rewrite upd_eq'.
+      repeat rewrite upd_ne; eauto.
+      destruct_lift H;
+        destruct_lift H1; cleanup.
+      intuition (eauto; try omega).
+      rewrite upd_ne; eauto.
+      omega.
+
+      intros; simpl.
+      norm; [cancel|].
+      eassign (upd dh 1 (Public, nat_to_value 0)).
+      rewrite nat_to_value_to_nat; eauto.
+      rewrite upd_eq'.
+      repeat rewrite upd_ne; eauto.
+      destruct_lift H;
+        destruct_lift H1; cleanup.
+      intuition (eauto; try omega).
+      rewrite upd_ne; eauto.
+      omega.
+    }
+    all: try solve [
+      intros; simpl in *;
+      destruct_lift H;
+        destruct_lift H1; cleanup;
+        norm; [cancel| intuition (eauto; try omega)]
+      ].
+  }
+
+  {
+      intros; simpl.
+      eapply hoare_triple_strengthen_pre.
+      eapply hoare_triple_weaken_post_strong.
+      eapply hoare_triple_weaken_crash_strong.
+      apply ret_okay.
+      eassign (((((0 |-> (Public, v, v0) ✶ F) ✶ 1 |-> v1) ✶ 2 |-> v2) ✶ ⟦⟦ r0 = v ⟧⟧)).
+      
+      intros; simpl; destruct_lift H; cleanup.
+      norm; [cancel| intuition (eauto; try omega)].
+
+      intros; simpl; destruct_lift H; cleanup.
+      norm; [cancel| intuition (eauto; try omega)].
+
+      intros; simpl; cancel.
+  }
+
+  all: try solve [
+       intros; simpl; destruct_lift H; cleanup;
+       norm; [cancel| intuition (eauto; try omega)]
+           ].
+Qed.
